\documentclass[12pt]{article}
\usepackage[utf8]{inputenc}
\usepackage[automark]{scrlayer-scrpage}
\usepackage[T1]{fontenc}
\usepackage[pdftex]{graphicx,color}
\usepackage{subcaption}
\usepackage{url}
\usepackage[pdftex,pdfpagelabels]{hyperref}
\usepackage[section,boxed]{algorithm}
\usepackage{algpseudocode}
\usepackage{amsmath}
\usepackage{amssymb}
\usepackage{amsthm}
\usepackage{lmodern}
\pagestyle{scrheadings}
\ofoot{}\cfoot{}\ifoot{}
\lehead{\pagemark}
\rehead{\slshape\leftmark}
\lohead{\slshape\leftmark}
\rohead{\pagemark}
\newtheorem{definition}{Definition}
\newtheorem{theorem}{Theorem}
\usepackage{blindtext}
\usepackage[margin=1in]{geometry} 
\usepackage{amsmath,amsthm,amssymb}
\usepackage{graphicx}
\newcommand{\N}{\mathbb{N}}
\newcommand{\Z}{\mathbb{Z}}
\newcommand{\R}{\mathbb{R}}
\newcommand{\C}{\mathbb{C}}
\newtheorem{thm}{Theorem}
\newcommand\myeq{\stackrel{\mathclap{\normalfont\mbox{IV}}}{=}}
\usepackage{mathtools}
\usepackage{amsmath}
 
\begin{document}
% --------------------------------------------------------------
%                         Title Page
% --------------------------------------------------------------
\title{Solutions for Sheet 2}
\author{Raphael Wude, Martin Br√ºckmann, Claude Jordan, Daniel Degenstein\\ \\
\textsc{Pattern Matching and Machine Learning} \\
\textsc{for Audio Signal Processing}}
\maketitle

% --------------------------------------------------------------
%                         Task 2.1
% --------------------------------------------------------------
\section*{Task 2.1}
\begin{thm} Let $1 \neq q \in \C$ then for all positive integers $n$: $\sum^{N-1}_{n=0}q^n = \frac{1-q^N}{1-q}$\end{thm}
\begin{proof}
Base Case $\left(N=1\right)$
$$\sum^{1-1}_{n=0}q^n = \sum^{0}_{n=0}q^n = q^0 = 1 = \frac{1-q}{1-q} = \frac{1-q^1}{1-q}$$
Inductive Step $\left(N \longrightarrow N+1\right)$
$$\sum^{N+1-1}_{n=0}q^n = \sum^{N}_{n=0}q^n = \sum^{N-1}_{n=0}q^n + q^N \myeq \frac{1-q^N}{1-q} + q^N = \frac{1-q^N}{1-q} + \frac{q^N\cdot (1-q)}{1-q} = \frac{1-q^N}{1-q} + \frac{q^N-q^{N+1}}{1-q} = \frac{1-q^N+q^N-q^{N+1}}{1-q} = \frac{1-q^{N+1}}{1-q}$$
\end{proof}

 
\end{document}