\documentclass[12pt]{article}
\usepackage[utf8]{inputenc}
\usepackage[automark]{scrlayer-scrpage}
\usepackage[T1]{fontenc}
\usepackage[pdftex]{graphicx,color}
\usepackage{subcaption}
\usepackage{url}
\usepackage[pdftex,pdfpagelabels]{hyperref}
\usepackage[section,boxed]{algorithm}
\usepackage{algpseudocode}
\usepackage{amsmath}
\usepackage{amssymb}
\usepackage{amsthm}
\usepackage{lmodern}
\pagestyle{scrheadings}
\ofoot{}\cfoot{}\ifoot{}
\lehead{\pagemark}
\rehead{\slshape\leftmark}
\lohead{\slshape\leftmark}
\rohead{\pagemark}
\newtheorem{definition}{Definition}
\newtheorem{theorem}{Theorem}
\usepackage{blindtext}
\usepackage[margin=1in]{geometry}
\usepackage{amsmath,amsthm,amssymb}
\usepackage{graphicx}
\newcommand{\N}{\mathbb{N}}
\newcommand{\Z}{\mathbb{Z}}
\newcommand{\R}{\mathbb{R}}
\newcommand{\C}{\mathbb{C}}
\newtheorem{thm}{Theorem}
\newcommand\myeq{\stackrel{\mathclap{\normalfont\mbox{IH}}}{=}}
\usepackage{mathtools}
\usepackage{amsmath}

\begin{document}
% --------------------------------------------------------------
%                         Title Page
% --------------------------------------------------------------
\title{Solutions for Sheet 2}
\author{Raphael Wude, Martin Br√ºckmann, Claude Jordan, Daniel Degenstein\\ \\
\textsc{Pattern Matching and Machine Learning} \\
\textsc{for Audio Signal Processing}}
\maketitle

% --------------------------------------------------------------
%                         Task 2.1
% --------------------------------------------------------------
\section*{Task 2.1}
\begin{thm} Let $1 \neq q \in \C$, then for all positive integers $n$: $\sum^{N-1}_{n=0}q^n = \frac{1-q^N}{1-q}$\end{thm}
\begin{proof}
Base Case $\left(N=1\right)$
$$\sum^{1-1}_{n=0}q^n
= \sum^{0}_{n=0}q^n
= q^0
= 1
= \frac{1-q}{1-q}
= \frac{1-q^1}{1-q}$$

Induction Hypothesis: Assume that for a given  $N$ the following statement holds:
$$\sum^{N-1}_{n=0}q^n = \frac{1-q^N}{1-q}$$

Inductive Step $\left(N \longrightarrow N+1\right)$
\begin{align*}
\sum^{N+1-1}_{n=0}q^n &= \sum^{N}_{n=0}q^n = \sum^{N-1}_{n=0}q^n + q^N \\
&\myeq \frac{1-q^N}{1-q} + q^N \\
&= \frac{1-q^N}{1-q} + \frac{q^N\cdot (1-q)}{1-q} \\
&= \frac{1-q^N}{1-q} + \frac{q^N-q^{N+1}}{1-q} \\
&= \frac{1-q^N+q^N-q^{N+1}}{1-q}\\
&= \frac{1-q^{N+1}}{1-q}
\end{align*}
\end{proof}

% --------------------------------------------------------------
%                         Task 2.3
% --------------------------------------------------------------
 \section*{Task 2.3}
 \begin{thm} Let $B = b_0,...,b_{N-1}$ denote an ON-basis of $\C^{N}$. Every ~$x \in \C^N$ has the following Fourier representation with respect to this ON-basis:
 $$x = \sum_{k=0}^{N-1} \langle x | b_k \rangle b_k$$.\end{thm}
 \begin{proof}
   Since B is a basis of $\C^N$, every vector $x \in \C^N$ can be written as follows:
   \begin{align*}
     x &= x_0 \cdot b_0 + x_1 \cdot b_1 + ... + x_{N-1} \cdot b_{N-1}\\
     &= \sum_{k=0}^{N-1}x_k \cdot b_k
   \end{align*}
   additionally for x_i, because ~$\langle b_i | b_i \rangle = 1$  for normalized vectors  and ~$\langle b_j | b_i \rangle = 0$ for $i,j \in \{0,...,N-1\} \wedge i \neq j$, stands:
   \begin{align*}
     x_i &= \langle b_i | b_i \rangle x_i = \langle b_i | b_i \rangle x_i + \sum_{k=0 \wedge k \neq i}^{N-1}\langle b_i | b_k \rangle x_k = 
      \sum_{k=0}^{N-1}x_k \cdot \langle b_i | b_k \rangle \\
     &= \sum_{k=0}^{N-1}\langle b_i | x_k \cdot b_k \rangle = \left\langle  b_i \middle | \sum_{k=0}^{N-1} x_k \cdot b_k \right\rangle
   \end{align*}
   And with the way to write a vector $x \in \C^N$ we get:
   \begin{align*}
     x_i = \langle b_i | x \rangle
   \end{align*}
   So all in all, we get for every vector $x \in \C^N$ the following representation:
   \begin{align*}
     x = \sum_{k=0}^{N-1}x_k \cdot b_k =  \sum_{k=0}^{N-1} \langle x | b_k \rangle b_k
   \end{align*}
 \end{proof}
\end{document}
